WIP better square

src/Experiments/NewPipeline/Arithmetic.v
@@ -1,5 +1,8 @@
 (* Following http://adam.chlipala.net/theses/andreser.pdf chapter 3 *)
+Require Import Crypto.Algebra.Nsatz.
 Require Import Coq.ZArith.ZArith Coq.micromega.Lia Crypto.Algebra.Nsatz.
+Require Import Coq.Sorting.Mergesort Coq.Structures.Orders.
+Require Import Coq.Sorting.Permutation.
 Require Import Coq.derive.Derive.
 Require Import Crypto.Util.Tactics.UniquePose Crypto.Util.Decidable.
 Require Import Crypto.Util.Tuple Crypto.Util.Prod Crypto.Util.LetIn.
@@ -28,6 +31,7 @@ Require Import Crypto.Util.Tactics.SplitInContext.
 Require Import Crypto.Util.Tactics.SubstEvars.
 Require Import Crypto.Util.Notations.
 Require Import Crypto.Util.ZUtil.Definitions.
+Require Import Crypto.Util.ZUtil.Sorting.
 Require Import Crypto.Util.ZUtil.CC Crypto.Util.ZUtil.Rshi.
 Require Import Crypto.Util.ZUtil.Zselect Crypto.Util.ZUtil.AddModulo.
 Require Import Crypto.Util.ZUtil.AddGetCarry Crypto.Util.ZUtil.MulSplit.
@@ -35,6 +39,7 @@ Require Import Crypto.Util.ZUtil Crypto.Util.ZUtil.Hints.Core.
 Require Import Crypto.Util.ZUtil.Modulo Crypto.Util.ZUtil.Div.
 Require Import Crypto.Util.ZUtil.Hints.PullPush.
 Require Import Crypto.Util.ZUtil.EquivModulo.
+Require Import Crypto.Util.Prod.
 Require Import Crypto.Util.CPSNotations.
 Require Import Crypto.Util.Equality.
 Import ListNotations. Local Open Scope Z_scope.
@@ -102,18 +107,36 @@ Module Associational.
     (* Goal: eval ?ab = eval [(100,(a1*b1));(10,a1*b0);(10,a0*b1);(1,a0*b0)]%RT *)
     trivial.                                              Defined.
 
+  Lemma eval_partition f (p:list (Z*Z)) :
+    eval (snd (partition f p)) + eval (fst (partition f p)) = eval p.
+  Proof. induction p; cbn [partition]; eta_expand; break_match; cbn [fst snd]; push; nsatz. Qed.
+  Hint Rewrite eval_partition : push_eval.
+
+  Lemma eval_partition' f (p:list (Z*Z)) :
+    eval (fst (partition f p)) + eval (snd (partition f p)) = eval p.
+  Proof. rewrite Z.add_comm, eval_partition; reflexivity. Qed.
+  Hint Rewrite eval_partition' : push_eval.
+
+  Lemma eval_fst_partition f p : eval (fst (partition f p)) = eval p - eval (snd (partition f p)).
+  Proof. rewrite <- (eval_partition f p); nsatz. Qed.
+  Lemma eval_snd_partition f p : eval (snd (partition f p)) = eval p - eval (fst (partition f p)).
+  Proof. rewrite <- (eval_partition f p); nsatz. Qed.
+
   Definition split (s:Z) (p:list (Z*Z)) : list (Z*Z) * list (Z*Z)
     := let hi_lo := partition (fun t => fst t mod s =? 0) p in
        (snd hi_lo, map (fun t => (fst t / s, snd t)) (fst hi_lo)).
-  Lemma eval_split s p (s_nz:s<>0) :
-    eval (fst (split s p)) + s * eval (snd (split s p)) = eval p.
-  Proof. cbv [Let_In split]; induction p;
+  Lemma eval_snd_split s p (s_nz:s<>0) :
+    s * eval (snd (split s p)) = eval (fst (partition (fun t => fst t mod s =? 0) p)).
+  Proof. cbv [split Let_In]; induction p;
     repeat match goal with
     | |- context[?a/?b] =>
       unique pose proof (Z_div_exact_full_2 a b ltac:(trivial) ltac:(trivial))
     | _ => progress push
     | _ => progress break_match
     | _ => progress nsatz                                end. Qed.
+  Lemma eval_split s p (s_nz:s<>0) :
+    eval (fst (split s p)) + s * eval (snd (split s p)) = eval p.
+  Proof. rewrite eval_snd_split, eval_fst_partition by assumption; cbv [split Let_In]; cbn [fst snd]; omega. Qed.
 
   Lemma reduction_rule a b s c (modulus_nz:s-c<>0) :
     (a + s * b) mod (s - c) = (a + c * b) mod (s - c).
@@ -129,6 +152,142 @@ Module Associational.
          rewrite <-reduction_rule, eval_split; trivial.      Qed.
   Hint Rewrite eval_reduce : push_eval.
 
+  Definition splitQ (s:Q) (p:list (Z*Z)) : list (Z*Z) * list (Z*Z)
+    := let hi_lo := partition (fun t => (fst t * Zpos (Qden s)) mod (Qnum s) =? 0) p in
+       (snd hi_lo, map (fun t => ((fst t * Zpos (Qden s)) / Qnum s, snd t)) (fst hi_lo)).
+  Lemma eval_snd_splitQ s p (s_nz:Qnum s<>0) :
+   Qnum s * eval (snd (splitQ s p)) = eval (fst (partition (fun t => (fst t * Zpos (Qden s)) mod (Qnum s) =? 0) p)) * Zpos (Qden s).
+  Proof.
+    (* Work around https://github.com/mit-plv/fiat-crypto/issues/381 ([nsatz] can't handle [Zpos]) *)
+    cbv [splitQ Let_In]; cbn [fst snd]; zify; generalize dependent (Zpos (Qden s)); generalize dependent (Qnum s); clear s; intros.
+    induction p;
+    repeat match goal with
+    | |- context[?a/?b] =>
+      unique pose proof (Z_div_exact_full_2 a b ltac:(trivial) ltac:(trivial))
+    | _ => progress push
+    | _ => progress break_match
+    | _ => progress nsatz                                end. Qed.
+  Lemma eval_splitQ s p (s_nz:Qnum s<>0) :
+    eval (fst (splitQ s p)) + (Qnum s * eval (snd (splitQ s p))) / Zpos (Qden s) = eval p.
+  Proof. rewrite eval_snd_splitQ, eval_fst_partition by assumption; cbv [splitQ Let_In]; cbn [fst snd]; Z.div_mod_to_quot_rem; nia. Qed.
+  Lemma eval_splitQ_mul s p (s_nz:Qnum s<>0) :
+    eval (fst (splitQ s p)) * Zpos (Qden s) + (Qnum s * eval (snd (splitQ s p))) = eval p * Zpos (Qden s).
+  Proof. rewrite eval_snd_splitQ, eval_fst_partition by assumption; cbv [splitQ Let_In]; cbn [fst snd]; nia. Qed.
+
+  Lemma eval_rev p : eval (rev p) = eval p.
+  Proof. induction p; cbn [rev]; push; lia. Qed.
+  Hint Rewrite eval_rev : push_eval.
+
+  Lemma eval_permutation (p q : list (Z * Z)) : Permutation p q -> eval p = eval q.
+  Proof. induction 1; push; nsatz.                          Qed.
+
+  Module RevWeightOrder <: TotalLeBool.
+    Definition t := (Z * Z)%type.
+    Definition leb (x y : t) := Z.leb (fst y) (fst x).
+    Infix "<=?" := leb.
+    Local Coercion is_true : bool >-> Sortclass.
+    Theorem leb_total : forall a1 a2, a1 <=? a2 \/ a2 <=? a1.
+    Proof.
+      cbv [is_true leb]; intros x y; rewrite !Z.leb_le; pose proof (Z.le_ge_cases (fst x) (fst y)).
+      omega.
+    Qed.
+    Global Instance leb_Transitive : Transitive leb.
+    Proof. repeat intro; unfold is_true, leb in *; Z.ltb_to_lt; omega. Qed.
+  End RevWeightOrder.
+
+  Module RevWeightSort := Mergesort.Sort RevWeightOrder.
+
+  Lemma eval_sort p : eval (RevWeightSort.sort p) = eval p.
+  Proof. symmetry; apply eval_permutation, RevWeightSort.Permuted_sort. Qed.
+  Hint Rewrite eval_sort : push_eval.
+
+  (* rough template (we actually have to do things a bit differently to account for duplicate weights):
+[ dlet fi_c := c * fi in
+   let (fj_high, fj_low) := split fj at s/fi.weight in
+   dlet fi_2 := 2 * fi in
+    dlet fi_2_c := 2 * fi_c in
+    (if fi.weight^2 >= s then fi_c * fi else fi * fi)
+       ++ fi_2_c * fj_high
+       ++ fi_2 * fj_low
+ | fi <- f , fj := (f weight less than i) ]
+   *)
+  (** N.B. We take advantage of dead code elimination to allow us to
+      let-bind partial products that we don't end up using *)
+  Definition reduce_square (s:Z) (c:list (Z*Z)) (p:list (Z*Z)) : list (Z*Z) :=
+    let two := [(1,2)] (* (weight, value) *) in
+    let p := RevWeightSort.sort p in (* now the highest weight limbs come first *)
+    list_rect
+      _
+      nil
+      (fun t ts acc
+       => (let hi_low_ts := partition (fun t' => (fst t * fst t') mod s =? 0) ts in
+          if ((snd t) * (snd t) <=? s)  (* reduce doesn't apply; no multiplication by [c] *)
+          then (dlet two_t2 := 2 * snd t in
+               (fst t * fst t, snd t * snd t)
+                 :: (map (fun t'
+                          => (fst t * fst t', two_t2 * snd t'))
+                         ts))
+          else (dlet c_t := mul [t] c in
+                dlet two_t := mul [t] two in
+                dlet two_c_t := mul c_t two in
+                (if ((snd t) * (snd t)) mod s =? 0 then [] else mul [t] [t])
+                  ++ mul two_t (snd hi_low_ts)
+                  ++ (map
+                        (fun t => (fst t / s, snd t))
+                        ((if ((snd t) * (snd t)) mod s =? 0 then mul c_t [t] else [])
+                           ++ mul two_c_t (fst hi_low_ts)))))
+           ++ acc)
+      p.
+  Lemma eval_reduce_square s c p (s_nz:s<>0) (modulus_nz:s-eval c<>0)
+    : eval (reduce_square s c p) mod (s - eval c)
+      = (eval p * eval p) mod (s - eval c).
+  Proof.
+    (*rewrite <- (eval_sort p).
+    cbv [reduce_square Let_In]; generalize (RevWeightSort.sort p) (RevWeightSort.StronglySorted_sort p _); clear p; intros p Hpsort.
+    induction Hpsort; cbn [list_rect]; push; [ nsatz | ].
+    rewrite Z.mul_add_distr_r, !Z.mul_add_distr_l, !Z.add_assoc.
+    apply Z.add_mod_Proper; cbv [Z.equiv_modulo]; [ clear IHHpsort | exact IHHpsort ].
+    break_innermost_match_step; Z.ltb_to_lt; push; [ f_equal; nsatz | ].
+
+    SearchAbout partition.
+
+    rewrite <- !Z.add_assoc; apply Z.add_mod_Proper; cbv [Z.equiv_modulo].
+
+    { break_match; Z.ltb_to_lt; push; try (f_equal; nsatz).
+
+      repeat match goal with H : context[Z.modulo] |- _ => revert H end.
+      Z.div_mod_to_quot_rem; nsatz.
+    break_match; push; try (f_equal; nsatz); Z.ltb_to_lt; autorewrite with zsimplify_const.
+
+
+    {
+      Focus 2.
+      rewrite ?(Z.mul_comm (fst _) (snd _)), <- !Z.mul_assoc.
+      Z.rewrite_mod_small.
+      push_Zmod;
+        rewrite <- Z.mul_mod_full; Z.rewrite_mod_small; pull_Zmod.
+
+      pull_Zmod.
+      SearchAbout ((_ mod _) * (_ mod _)).
+
+      SearchAbout
+
+    cbn [mul map].
+    2:apply IHHpsort.
+    rewrite Z
+    break_innermost_match; Z.ltb_to_lt; push.
+
+    cbn [filter].
+    SearchAbout filter cons.
+    apply Z.add_mod_Proper; cbv [Z.equiv_modulo].
+    Focus 2.
+    2:
+    SearchAbout Proper Z.equiv_modulo.
+    SearchAbout ((_ + _) mod _).
+    eta_expand; push.
+                                                         nsatz.*)Admitted.
+  Hint Rewrite eval_reduce_square : push_eval.
+
   Definition bind_snd (p : list (Z*Z)) :=
     map (fun t => dlet_nd t2 := snd t in (fst t, t2)) p.
 
@@ -137,9 +296,6 @@ Module Associational.
     cbv [bind_snd]; induction p as [| [? ?] ];
       push; [|rewrite IHp]; reflexivity.
   Qed.
-
-  Lemma eval_rev p : eval (rev p) = eval p.
-  Proof. induction p; cbn [rev]; push; lia. Qed.
 
   Section Carries.
     Definition carryterm (w fw:Z) (t:Z * Z) :=
@@ -308,17 +464,14 @@ Module Positional. Section Positional.
 
     Definition squaremod (n:nat) (a:list Z) : list Z
       := let a_a := to_associational n a in
-         let aa_a := Associational.square a_a in
-         let aam_a := Associational.reduce s c aa_a in
-         from_associational n aam_a.
+         let aa_a := Associational.reduce_square s c a_a in
+         from_associational n aa_a.
     Lemma eval_squaremod n (f:list Z)
           (Hf : length f = n) :
       eval n (squaremod n f) mod (s - Associational.eval c)
       = (eval n f * eval n f) mod (s - Associational.eval c).
     Proof. cbv [squaremod]; push; trivial.
-    destruct f; simpl in *; [ right; subst n | left; try omega.. ].
-    clear; cbv -[Associational.reduce].
-    induction c as [|?? IHc]; simpl; trivial.                 Qed.
+    destruct f; simpl in *; [ right; subst n; reflexivity | left; try omega.. ]. Qed.
   End mulmod.
   Hint Rewrite @eval_mulmod @eval_squaremod : push_eval.
 
